Functions to construct umvec-cmvec from a state, progress on cfi stopping

cfi/symbolic.v
@@ -5,6 +5,7 @@ Require Import ssreflect ssrfun ssrbool eqtype ssrnat.
 Require Import lib.utils lib.partial_maps.
 Require Import common.common.
 Require Import symbolic.symbolic.
+Require Import symbolic.exec.
 Require Import cfi.property.
 Require Import cfi.rules.
 Require Import lib.Coqlib.
@@ -492,76 +493,19 @@ Program Instance symbolic_cfi_machine : cfi_machine := {|
 Import DoNotation.
 Import Vector.VectorNotations.
 
-(*TODO: Move to symbolic*)
-Definition build_mvec st : option (Symbolic.MVec (Symbolic.tag t)) :=
-  let '(Symbolic.State mem reg pc@tpc int) := st in
-  match get mem pc with
-    | Some i =>
-      match decode_instr (common.val i) with
-        | Some op =>
-          let part := @Symbolic.mkMVec (Symbolic.tag t) (opcode_of op) tpc (tag i) in
-          match op return (Symbolic.mvec_operands (Symbolic.tag t) (Symbolic.nfields (opcode_of op)) ->
-                           Symbolic.MVec (Symbolic.tag t)) -> option (Symbolic.MVec (Symbolic.tag t)) with
-            | Nop => fun part => Some (part [])
-            | Const n r => fun part => 
-                do! old <- get reg r;
-                Some (part [tag old])
-            | Mov r1 r2 => fun part =>
-              do! v1 <- get reg r1;
-              do! v2 <- get reg r2;
-              Some (part [(tag v1); (tag v2)])
-            | Binop _ r1 r2 r3 => fun part =>
-              do! v1 <- get reg r1;
-              do! v2 <- get reg r2;
-              do! v3 <- get reg r3;
-              Some (part [(tag v1); (tag v2); (tag v3)])
-            | Load  r1 r2 => fun part =>
-              do! w1 <- get reg r1;
-              do! w2 <- get mem (val w1);
-              do! old <- get reg r2;
-              Some (part [(tag w1); (tag w2); (tag old)])
-            | Store  r1 r2 => fun part =>
-              do! w1 <- get reg r1;
-              do! w2 <- get reg r2;
-              do! w3 <- get mem (val w1);
-              Some (part [(tag w1); (tag w1); (tag w3)])
-            | Jump  r => fun part =>
-              do! w <- get reg r;
-              Some (part [tag w])
-            | Bnz  r n => fun part =>
-              do! w <- get reg r;
-              Some (part [tag w])
-            | Jal  r => fun part =>
-              do! w <- get reg r;
-              do! old <- get reg ra;
-              Some (part [tag w; tag old])
-            | JumpEpc => fun _ => None
-            | AddRule => fun _ => None
-            | GetTag _ _ => fun _ => None
-            | PutTag _ _ _ => fun _ => None
-            | Halt => fun _ => None
-          end part
-        | None => None
-      end
-    | None => 
-      match Symbolic.get_syscall table pc with
-        | Some sc =>
-          Some (@Symbolic.mkMVec (Symbolic.tag _) SERVICE tpc (Symbolic.entry_tag sc) (Vector.nil _))
-        | None => None
-      end 
-  end.
-
 Definition option_handler x := 
   match x with
     | Some v => Symbolic.handler v
     | None => None
   end.
 
+(*If we have a violation then the symbolic handler will
+ say no*)
 Lemma succ_false_handler asi asj :
   invariants asi ->
   ssucc asi asj = false ->
   step asi asj ->
-  option_handler (build_mvec asj) = None.
+  option_handler (build_mvec table asj) = None.
 Proof.
   intros INV SUCC STEP.
   unfold ssucc in SUCC.
