cfi/concrete.v
@@ -116,25 +116,6 @@ Definition csucc (st : Concrete.state t) (st' : Concrete.state t) : bool :=
       end
     | None => false
   end.
-(*
-Definition csucc (st : Concrete.state t) (st' : Concrete.state t) : bool :=
-  let pc_s := common.val (Concrete.pc st) in
-  let pc_s' := common.val (Concrete.pc st') in
-  if in_kernel st || in_kernel st' then true else
-  match (get (Concrete.mem st) pc_s) with
-    | Some i =>
-      if (common.tag i) == encode (USER DATA) then false
-      else
-        match decode_instr (common.val i) with
-          | Some (Jump r) => valid_jmp pc_s pc_s'
-          | Some (Jal r) => valid_jmp pc_s pc_s'
-          | Some (Bnz r imm) => 
-            (pc_s' == pc_s .+1) || (pc_s' == pc_s + imm_to_word imm)
-          | None => false
-          | _ => pc_s' == pc_s .+1
-      end
-    | None => false
-  end. *)
 
 Definition sp := @Sym.sym_cfi t _ _ _ _ valid_jmp.
 
